update

src/canonize/norm.lean
@@ -2,9 +2,9 @@ import .sterm .pterm
 
 namespace polya
 
-inductive alt {γ} [const_space γ] : Type
-| sform : list (@nterm γ _) → @sterm γ _ → alt
-| pform : list (@nterm γ _) → @pterm γ _ → alt
+inductive alt {γ} [const_space γ] : bool → Type
+| sform : list (@nterm γ _) → @sterm γ _ → alt tt
+| pform : list (@nterm γ _) → @pterm γ _ → alt ff
 
 namespace alt
 open nterm
@@ -13,110 +13,137 @@ variables {α : Type} [discrete_field α]
 variables {γ : Type} [const_space γ]
 variables [morph γ α] {ρ : dict α}
 
-def singleton (x : @nterm γ _) : @alt γ _ :=
-sform [] (sterm.singleton x)
+def singleton (x : @nterm γ _) : Π {b}, @alt γ _ b
+| tt := sform [] (sterm.singleton x)
+| ff := pform [] (pterm.singleton x)
 
-def to_nterm : @alt γ _ → @nterm γ _
-| (sform _ S) := S.to_nterm
-| (pform _ P) := P.to_nterm
+def to_nterm : Π {b}, @alt γ _ b → @nterm γ _
+| ._ (sform _ S) := S.to_nterm
+| ._ (pform _ P) := P.to_nterm
 
-def hyps : @alt γ _ → list (@nterm γ _)
-| (sform l _) := l
-| (pform l _) := l
-
-def eval (ρ : dict α) (x : @alt γ _) : α :=
-nterm.eval ρ x.to_nterm
-
-theorem eval_def {x : @alt γ _} : eval ρ x = nterm.eval ρ x.to_nterm := rfl
-
-def reduce : @alt γ _ → @alt γ _
-| (sform l S) := sform l S.reduce
-| (pform l P) := pform (l ∪ P.reduce_hyps) P.reduce
-
-def reduce_hyps : @alt γ _ → list (@nterm γ _)
-| (sform l S) := []
-| (pform l P) := P.reduce_hyps
-
-def to_sterm : @alt γ _ → @sterm γ _
+def to_sterm : @alt γ _ tt → @sterm γ _
 | (sform _ S) := S
-| x := sterm.of_nterm x.to_nterm
 
-def to_pterm : @alt γ _ → @pterm γ _
+def to_pterm : @alt γ _ ff → @pterm γ _
 | (pform _ P) := P
-| x := pterm.of_nterm x.to_nterm
 
-theorem eval_singleton {x : @nterm γ _} :
-  eval ρ (singleton x) = nterm.eval ρ x :=
+def hyps : Π {b}, @alt γ _ b → list (@nterm γ _)
+| ._ (sform ts _) := ts
+| ._ (pform ts _) := ts
+
+def eval (ρ : dict α) : Π {b}, @alt γ _ b → α
+| ._ (sform _ S) := sterm.eval ρ S
+| ._ (pform _ P) := pterm.eval ρ P
+
+def to_sform : Π {b}, @alt γ _ b → @alt γ _ tt
+| ._ (sform ts S) := sform ts S
+| ._ (pform ts P) := sform (ts ∪ P.reduce_hyps) (sterm.of_nterm P.reduce.to_nterm)
+
+def to_pform : Π {b}, @alt γ _ b → @alt γ _ ff
+| ._ (sform ts S) := pform ts (pterm.of_nterm S.to_nterm)
+| ._ (pform ts P) := pform ts P
+
+def hyps_to_sform {b} {x : @alt γ _ b} :
+  x.hyps ⊆ x.to_sform.hyps :=
 begin
-  unfold singleton, unfold eval, unfold to_nterm,
-  rw [← sterm.eval_to_nterm, sterm.eval_singleton]
+  sorry
 end
 
-theorem eval_reduce {x : @alt γ _} :
-  nonzero ρ x.reduce_hyps →
-  eval ρ x.reduce = eval ρ x :=
+theorem eval_def {b} {x : @alt γ _ b} :
+  eval ρ x = nterm.eval ρ x.to_nterm :=
 begin
-  intro H,
-  cases x with l S l P,
-  { unfold reduce, unfold eval, unfold to_nterm,
-    rw [← sterm.eval_to_nterm, ← sterm.eval_reduce, sterm.eval_to_nterm] },
-  { unfold reduce, unfold eval, unfold to_nterm,
-    rw [← pterm.eval_to_nterm, ← pterm.eval_reduce H, pterm.eval_to_nterm] }
+cases x with ts S,
+  { simp [eval, to_nterm, sterm.eval_to_nterm] },
+  { simp [eval, to_nterm, pterm.eval_to_nterm] }
 end
 
-theorem eval_to_sterm {x : @alt γ _} :
-  eval ρ x = sterm.eval ρ x.to_sterm :=
+theorem eval_singleton {b} {x : @nterm γ _} :
+  eval ρ (singleton x : @alt γ _ b) = nterm.eval ρ x :=
 begin
-  cases x,
-  { unfold to_sterm, unfold eval, unfold to_nterm, rw ← sterm.eval_to_nterm },
-  { unfold to_sterm, unfold eval, unfold to_nterm, rw ← sterm.eval_of_nterm }
+  cases b,
+  { unfold singleton, unfold eval,
+    rw ← pterm.eval_singleton },
+  { unfold singleton, unfold eval,
+    rw ← sterm.eval_singleton }
 end
 
-theorem eval_to_pterm {x : @alt γ _} :
+theorem eval_to_sform {b} {x : @alt γ _ b} :
+  nonzero ρ x.to_sform.hyps →
+  eval ρ x.to_sform = eval ρ x :=
+begin
+  sorry
+end
+
+theorem eval_to_sterm {x : @alt γ _ tt} :
+  sterm.eval ρ x.to_sterm = eval ρ x :=
+begin
+  cases x, unfold to_sterm, unfold eval
+end
+
+theorem eval_to_pterm {x : @alt γ _ ff} :
   eval ρ x = pterm.eval ρ x.to_pterm :=
 begin
-  cases x,
-  { unfold to_pterm, unfold eval, unfold to_nterm, rw ← pterm.eval_of_nterm },
-  { unfold to_pterm, unfold eval, unfold to_nterm, rw ← pterm.eval_to_nterm }
+  cases x, unfold to_pterm, unfold eval
 end
 
-def add (x y : @alt γ _) : @alt γ _ :=
+--TODO:
+--more cases to avoid switching form too often
+--when applying operators
+
+def add_sform (x y : @alt γ _ tt) : @alt γ _ tt :=
 sform (x.hyps ∪ y.hyps) (x.to_sterm + y.to_sterm)
---TODO: more cases to avoid switching form too often
 
-def mul (x y : @alt γ _) : @alt γ _ :=
+def mul_pform (x y : @alt γ _ ff) : @alt γ _ ff :=
 pform (x.hyps ∪ y.hyps) (x.to_pterm * y.to_pterm)
---TODO: more cases to avoid switching form too often
 
-def pow (x : @alt γ _) (n : znum) : @alt γ _ :=
+def pow_pform (x : @alt γ _ ff) (n : znum) : @alt γ _ ff :=
 if n = 0 then singleton (1 : γ)
-else if n = 1 then x
 else pform x.hyps (x.to_pterm ^ n)
 
-instance : has_add (@alt γ _) := ⟨add⟩
-instance : has_mul (@alt γ _) := ⟨mul⟩
-instance : has_pow (@alt γ _) znum := ⟨pow⟩
+instance : has_add (@alt γ _ tt) := ⟨add_sform⟩
+instance : has_mul (@alt γ _ ff) := ⟨mul_pform⟩
+instance : has_pow (@alt γ _ ff) znum := ⟨pow_pform⟩
 
-@[simp] theorem hyps_add {x y : @alt γ _} :
+def add {a b} (x : @alt γ _ a) (y : @alt γ _ b) : @alt γ _ tt :=
+x.to_sform + y.to_sform
+
+def mul {a b} (x : @alt γ _ a) (y : @alt γ _ b) : @alt γ _ ff :=
+x.to_pform * y.to_pform
+
+def pow {a} (x : @alt γ _ a) (n : znum) : @alt γ _ ff :=
+x.to_pform ^ n
+
+theorem hyps_singleton {b} {x : @nterm γ _} :
+  (singleton x : @alt γ _ b).hyps = [] :=
+by cases b; simp [singleton, hyps]
+
+theorem hyps_add_sform {x y : @alt γ _ tt} :
   (x + y).hyps = x.hyps ∪ y.hyps :=
-by { simp [hyps, has_add.add, add] }
+by simp [has_add.add, add_sform, hyps] 
 
-@[simp] theorem hyps_mul {x y : @alt γ _} :
+theorem hyps_mul_pform {x y : @alt γ _ ff} :
   (x * y).hyps = x.hyps ∪ y.hyps :=
-by { simp [hyps, has_mul.mul, mul] }
+by simp [has_mul.mul, mul_pform, hyps]
 
-@[simp] theorem hyps_pow {x : @alt γ _} {n : znum} :
+theorem hyps_pow_pform {x : @alt γ _ ff} {n : znum} :
   (x ^ n).hyps = if n = 0 then [] else x.hyps :=
 begin
   by_cases h0 : n = 0;
   by_cases h1 : n = 1;
-  simp [h0, h1, has_pow.pow, pow, hyps, singleton]
+  simp [has_pow.pow, pow_pform, h0, h1, hyps, hyps_singleton]
 end
 
-def of_nterm : @nterm γ _ → @alt γ _
-| (nterm.add x y) := of_nterm x + of_nterm y
-| (nterm.mul x y) := of_nterm x * of_nterm y
-| (nterm.pow x n) := of_nterm x ^ n
+@[reducible]
+def aux_of_nterm : @nterm γ _ → bool
+| (nterm.add _ _) := tt
+| (nterm.mul _ _) := ff
+| (nterm.pow _ _) := ff
+| _ := tt
+
+def of_nterm : Π (x : @nterm γ _), @alt γ _ (aux_of_nterm x)
+| (nterm.add x y) := add (of_nterm x) (of_nterm y)
+| (nterm.mul x y) := mul (of_nterm x) (of_nterm y)
+| (nterm.pow x n) := pow (of_nterm x) n
 | x := singleton x
 
 theorem eval_of_nterm {x : @nterm γ _} :
@@ -126,7 +153,9 @@ begin
   induction x with i c x y ihx ihy x y ihx ihy x n ihx,
   { intro, unfold of_nterm, rw eval_singleton },
   { intro, unfold of_nterm, rw eval_singleton },
-  repeat {sorry}
+  { sorry },
+  { sorry },
+  { sorry }
 end
 
 end alt
@@ -138,20 +167,23 @@ variables {γ : Type} [const_space γ]
 variables [morph γ α] {ρ : dict α}
 
 def norm (x : @nterm γ _) : @nterm γ _ :=
-(alt.of_nterm x).to_nterm
+(alt.of_nterm x).to_sform.to_nterm
 
 def norm_hyps (x : @nterm γ _) : list (@nterm γ _) :=
-(alt.of_nterm x).hyps
+(alt.of_nterm x).to_sform.hyps
 
 def correctness {x : @nterm γ _} :
   nonzero ρ (norm_hyps x) →
-  nterm.eval ρ x = nterm.eval ρ (norm x) :=
+  nterm.eval ρ (norm x) = nterm.eval ρ x :=
 begin
-  sorry
+  intro H, unfold norm,
+  rw [← alt.eval_def, ← alt.eval_of_nterm, alt.eval_to_sform],
+  { intros t ht, apply H, exact ht },
+  { intros t ht, apply H, apply alt.hyps_to_sform, exact ht }
 end
 
 def naive_norm : @nterm γ _ → @nterm γ _
-| (add x y) := (sterm.of_nterm (naive_norm x) + sterm.of_nterm (naive_norm y)).reduce.to_nterm
+| (add x y) := (sterm.of_nterm (naive_norm x) + sterm.of_nterm (naive_norm y)).to_nterm
 | (mul x y) := (pterm.of_nterm (naive_norm x) * pterm.of_nterm (naive_norm y)).reduce.to_nterm
 | (pow x n) := (pterm.of_nterm (naive_norm x) ^ n).reduce.to_nterm
 | x := x
@@ -160,6 +192,9 @@ theorem soundness {x : @nterm γ _} :
   norm x = naive_norm x :=
 begin
   sorry
+  --TODO: this theorem is not required,
+  --but it could be an interesting
+  --first step to prove soundness
 end
 
 end nterm
