src/canonize/test.lean
@@ -6,8 +6,9 @@ open tactic polya
 set_option trace.check true
 meta def test (e : expr) : tactic unit :=
 do
-    (nt, new_e, pr) ← norm_expr e,
+    (new_e, hyps) ← test_norm e,
     trace new_e,
+    trace hyps,
     skip
 
 constants u v w x y z : ℝ
@@ -28,8 +29,8 @@ run_cmd test `( x * y * z * (3 : ℚ) - z * x * y * (4 : ℚ) )
 run_cmd test `( x * ((y * w) * (z * (u * z) * v) * w) )
 run_cmd test `( (x * (2 : ℚ)) * ((3 : ℚ) / x) )
 run_cmd test `( (x * y) ^ 3 / x ^ 2 )
+run_cmd test `( (x - y + y) * z )
 run_cmd test `( (x / x) ^ 0 )
 run_cmd test `( (x + y) ^ 2 / (x + y) ^ 2 * x * y / x )
 run_cmd test `( x ^ 4 )
 
-run_cmd test `( (x + y) / (y + x) )
